src/SMT_terms.v
@@ -41,7 +41,8 @@ Module Form.
   | Fimp (_:fargs)
   | Fxor (_:_lit) (_:_lit)
   | Fiff (_:_lit) (_:_lit)
-  | Fite (_:_lit) (_:_lit) (_:_lit).
+  | Fite (_:_lit) (_:_lit) (_:_lit)
+  | Fand_int (_:fargs).
 
   Definition is_Ftrue h :=
     match h with Ftrue => true | _ => false end.
@@ -80,6 +81,7 @@ Module Form.
         | Fite a b c =>
           if Lit.interp interp_var a then Lit.interp interp_var b
           else Lit.interp interp_var c
+        | Fand_int args => afold_left _ _ max_int land (Lit.interp interp_var) args
         end.
 
     End Interp_form.
